VCVio/OracleComp/Coercions/Append.lean
@@ -14,15 +14,15 @@ in the sense that the two oracle sets correspond to `Sum.inl` and `Sum.inr`.
 Note that this operation is never associative, as `Sum` is not associative
 
 We also define a number of coercions involving append.
-These instances allow an `OracleSpec` of the form `spec₁ ++ ... ++ spec₂`
-to coerce to one of the form `spec'₁ ++ ... ++ spec'₂`, assuming that
+These instances allow an `OracleSpec` of the form `spec₁ ++ₒ ... ++ₒ spec₂`
+to coerce to one of the form `spec'₁ ++ₒ ... ++ₒ spec'₂`, assuming that
 the set of oracles in the first is a sub-sequence of the oracles in the second.
 We also include associativity instances, so parenthisization of the sequence is irrelevant.
 
 Note that this requires the ordering of oracles in each to match,
 and so we generally adopt a standard ordering of `OracleSpec` for computations
 in order to make this apply as often as possible. We specifically adopt the following convention:
-  `{coin_oracle} ++ {unif_spec} ++ {random oracle} ++ {adversary oracles} ++ ...`,
+  `{coin_oracle} ++ₒ {unif_spec} ++ₒ {random oracle} ++ₒ {adversary oracles} ++ₒ ...`,
 where any of the individual parts may be ommited. The adversary oracles are for
 things like a signing oracle in unforgeability experiments of a signature scheme.
 
@@ -42,21 +42,71 @@ open OracleComp Sum
 
 namespace OracleSpec
 
-variable {ι₁ ι₂ : Type} (spec₁ : OracleSpec ι₁) (spec₂ : OracleSpec ι₂)
+variable {ι₁ ι₂ ι₃ ι₄: Type} (spec₁ : OracleSpec ι₁) (spec₂ : OracleSpec ι₂)
+  (spec₃ : OracleSpec ι₃) (spec₄ : OracleSpec ι₄) {α β γ : Type}
 
 section instances
 
+/-- Add additional oracles to the right side of the existing ones. -/
 instance subSpec_append_left : spec₁ ⊂ₒ (spec₁ ++ₒ spec₂) where
   toFun := λ i t ↦ query (inl i) t
   evalDist_toFun' := by simp [append]
-instance {α : Type} : Coe (OracleComp spec₁ α) (OracleComp (spec₁ ++ₒ spec₂) α)
-  where coe := liftComp
 
+instance : Coe (OracleComp spec₁ α) (OracleComp (spec₁ ++ₒ spec₂) α) where
+  coe := liftComp
+
+/-- Add additional oracles to the left side of the exiting ones-/
 instance subSpec_append_right : spec₂ ⊂ₒ (spec₁ ++ₒ spec₂) where
   toFun := λ i t ↦ query (inr i) t
   evalDist_toFun' := by simp [append]
-instance {α : Type} : Coe (OracleComp spec₂ α) (OracleComp (spec₁ ++ₒ spec₂) α)
-  where coe := liftComp
+
+instance : Coe (OracleComp spec₂ α) (OracleComp (spec₁ ++ₒ spec₂) α) where
+  coe := liftComp
+
+/-- Using a existing `subSpec`, also expand to even more additional oracles on the left. -/
+instance subSpec_append_left_of_subSpec [h : spec₁ ⊂ₒ spec₃] : spec₁ ⊂ₒ (spec₂ ++ₒ spec₃) where
+  toFun := λ i t ↦ liftComp (h.toFun i t)
+  evalDist_toFun' := sorry
+
+  /-- Using a existing `subSpec`, also expand to even more additional oracles on the right. -/
+instance subSpec_append_right_of_subSpec [h : spec₁ ⊂ₒ spec₂] : spec₁ ⊂ₒ (spec₂ ++ₒ spec₃) where
+  toFun := λ i t ↦ liftComp (h.toFun i t)
+  evalDist_toFun' := sorry
+
+instance subSpec_left_append_left_append_of_subSpec [h : spec₁ ⊂ₒ spec₃] :
+    spec₁ ++ₒ spec₂ ⊂ₒ spec₃ ++ₒ spec₂ where
+  toFun := λ i t ↦ match i with
+    | inl i => liftComp (h.toFun i t)
+    | inr i => query (inr i) t
+  evalDist_toFun' := sorry
+
+instance subSpec_right_append_right_append_of_subSpec [h : spec₂ ⊂ₒ spec₃] :
+    spec₁ ++ₒ spec₂ ⊂ₒ spec₁ ++ₒ spec₃ where
+  toFun := λ i t ↦ match i with
+    | inl i => query (inl i) t
+    | inr i => liftComp (h.toFun i t)
+  evalDist_toFun' := sorry
+
+
+
+-- instance{ι₁ : Type} {ι₂ : Type} {ι₃ : Type}
+--   (spec₁ : OracleSpec ι₁)
+--   (spec₂ : OracleSpec ι₂)
+--   (spec₃ : OracleSpec ι₃) {α : Type}
+--   [spec₂ ⊂ₒ spec₃] : Coe (OracleComp spec₂ α) (OracleComp (spec₁ ++ₒ spec₃) α) where
+--   coe := liftComp
+
+
+instance subSpec_assoc : spec₁ ++ₒ (spec₂ ++ₒ spec₃) ⊂ₒ spec₁ ++ₒ spec₂ ++ₒ spec₃ where
+  toFun := λ i t ↦ match i with
+    | inl i => query (inl (inl i)) t
+    | inr (inl i) => query (inl (inr i)) t
+    | inr (inr i) => query (inr i) t
+  evalDist_toFun' := sorry
+
+instance : Coe (OracleComp (spec₁ ++ₒ (spec₂ ++ₒ spec₃)) α)
+    (OracleComp (spec₁ ++ₒ spec₂ ++ₒ spec₃) α) where
+  coe := liftComp
 
 end instances
 
@@ -64,24 +114,82 @@ end OracleSpec
 
 section tests
 
-variable {spec₁ spec₂ spec₃ spec₄}
+-- -- This set of examples serves as sort of a "unit test" for the coercions above
+-- variables (α ι₁ ι₂ ι₃ ι₄ ι₅ ι₆ : Type)
+--   (spec₁ : OracleSpec ι₁) (spec₂ : OracleSpec ι₂)
+--   (spec₃ : OracleSpec ι₃) (spec₄ : OracleSpec ι₄)
+--   (coeSpec : OracleSpec ι₅) (coeSuperSpec : OracleSpec ι₆)
+--   [coeSpec ⊂ₒ coeSuperSpec]
 
--- This set of examples serves as sort of a "unit test" for the coercions above
-variable (α : Type) {ι1 ι2 ι3 ι4 ι5 ι6 : Type}
-  (spec : OracleSpec ι1)
-  (spec' : OracleSpec ι2)
-  (spec'' : OracleSpec ι3)
-  (spec''' : OracleSpec ι4)
-  (coe_spec : OracleSpec ι5)
-  (coe_spec' : OracleSpec ι6)
-  [coe_spec ⊂ₒ coe_spec']
+-- -- coerce a single `coin_spec` and then append extra oracles
+-- example (oa : OracleComp coeSpec α) :
+--   OracleComp (coeSuperSpec ++ₒ spec₂ ++ₒ spec₃) α := liftComp oa
+-- example (oa : OracleComp coeSpec α) :
+--   OracleComp (spec₁ ++ₒ coeSuperSpec ++ₒ spec₂) α := liftComp oa
+-- example (oa : OracleComp coeSpec α) :
+--   OracleComp (spec₁ ++ₒ spec₂ ++ₒ coeSuperSpec) α := liftComp oa
 
--- coerce a single `coin_spec` and then append extra oracles
-example [coe_spec ⊂ₒ coe_spec'] (oa : OracleComp coe_spec α) :
-  OracleComp (coe_spec ++ₒ spec') α := ↑oa
-example (oa : OracleComp coe_spec α) :
-  OracleComp (spec ++ₒ coe_spec ++ₒ spec') α := ↑oa
-example (oa : OracleComp coe_spec α) :
-  OracleComp (spec ++ₒ spec' ++ₒ coe_spec) α := ↑oa
+-- -- coerce left side of append and then append on additional oracles
+-- example (oa : OracleComp (coeSpec ++ₒ spec₁) α) :
+--   OracleComp (coeSuperSpec ++ₒ spec₁ ++ₒ spec₂) α := ↑oa
+-- example (oa : OracleComp (coeSpec ++ₒ spec₁) α) :
+--   OracleComp (coeSuperSpec ++ₒ spec₂ ++ₒ spec₁) α := ↑oa
+-- example (oa : OracleComp (coeSpec ++ₒ spec₁) α) :
+--   OracleComp (spec₂ ++ₒ coeSuperSpec ++ₒ spec₁) α := ↑oa
+
+-- -- coerce right side of append and then append on additional oracles
+-- example (oa : OracleComp (spec₁ ++ₒ coeSpec) α) :
+--   OracleComp (spec₁ ++ₒ coeSuperSpec ++ₒ spec₂) α := ↑oa
+-- example (oa : OracleComp (spec₁ ++ₒ coeSpec) α) :
+--   OracleComp (spec₁ ++ₒ spec₂ ++ₒ coeSuperSpec) α := ↑oa
+-- example (oa : OracleComp (spec₁ ++ₒ coeSpec) α) :
+--   OracleComp (spec₂ ++ₒ spec₁ ++ₒ coeSuperSpec) α := ↑oa
+
+-- -- coerce an inside part while also applying associativity
+-- example (oa : OracleComp (spec₁ ++ₒ (spec₂ ++ₒ coeSpec)) α) :
+--   OracleComp (spec₁ ++ₒ spec₂ ++ₒ coeSuperSpec) α := ↑oa
+-- example (oa : OracleComp (spec₁ ++ₒ (coeSpec ++ₒ spec₂)) α) :
+--   OracleComp (spec₁ ++ₒ coeSuperSpec ++ₒ spec₂) α := ↑oa
+-- example (oa : OracleComp (coeSpec ++ₒ (spec₁ ++ₒ spec₂)) α) :
+--   OracleComp (coeSuperSpec ++ₒ spec₁ ++ₒ spec₂) α := ↑oa
+
+-- -- coerce two oracles up to four oracles
+-- example (oa : OracleComp (spec₁ ++ₒ spec₂) α) :
+--   OracleComp (spec₁ ++ₒ spec₂ ++ₒ spec₃ ++ₒ spec₄) α := ↑oa
+-- example (oa : OracleComp (spec₁ ++ₒ spec₃) α) :
+--   OracleComp (spec₁ ++ₒ spec₂ ++ₒ spec₃ ++ₒ spec₄) α := ↑oa
+-- example (oa : OracleComp (spec₁ ++ₒ spec₄) α) :
+--   OracleComp (spec₁ ++ₒ spec₂ ++ₒ spec₃ ++ₒ spec₄) α := ↑oa
+-- example (oa : OracleComp (spec₂ ++ₒ spec₃) α) :
+--   OracleComp (spec₁ ++ₒ spec₂ ++ₒ spec₃ ++ₒ spec₄) α := ↑oa
+-- example (oa : OracleComp (spec₂ ++ₒ spec₄) α) :
+--   OracleComp (spec₁ ++ₒ spec₂ ++ₒ spec₃ ++ₒ spec₄) α := ↑oa
+-- example (oa : OracleComp (spec₃ ++ₒ spec₄) α) :
+--   OracleComp (spec₁ ++ₒ spec₂ ++ₒ spec₃ ++ₒ spec₄) α := ↑oa
+
+-- -- coerce threee oracles up to four oracles
+-- example (oa : OracleComp (spec₁ ++ₒ spec₂ ++ₒ spec₃) α) :
+--   OracleComp (spec₁ ++ₒ spec₂ ++ₒ spec₃ ++ₒ spec₄) α := ↑oa
+-- example (oa : OracleComp (spec₁ ++ₒ spec₂ ++ₒ spec₄) α) :
+--   OracleComp (spec₁ ++ₒ spec₂ ++ₒ spec₃ ++ₒ spec₄) α := ↑oa
+-- example (oa : OracleComp (spec₁ ++ₒ spec₃ ++ₒ spec₄) α) :
+--   OracleComp (spec₁ ++ₒ spec₂ ++ₒ spec₃ ++ₒ spec₄) α := ↑oa
+-- example (oa : OracleComp (spec₂ ++ₒ spec₃ ++ₒ spec₄) α) :
+--   OracleComp (spec₁ ++ₒ spec₂ ++ₒ spec₃ ++ₒ spec₄) α := ↑oa
+
+-- -- four oracles with associativity and internal coercion
+-- example (oa : OracleComp ((coeSpec ++ₒ spec₂) ++ₒ (spec₃ ++ₒ spec₄)) α) :
+--   OracleComp (coeSuperSpec ++ₒ spec₂ ++ₒ spec₃ ++ₒ spec₄) α := ↑oa
+-- example (oa : OracleComp ((spec₁ ++ₒ spec₂) ++ₒ (coeSpec ++ₒ spec₄)) α) :
+--   OracleComp (spec₁ ++ₒ spec₂ ++ₒ coeSuperSpec ++ₒ spec₄) α := ↑oa
+-- example (oa : OracleComp ((spec₁ ++ₒ coeSpec) ++ₒ (spec₃ ++ₒ spec₄)) α) :
+--   OracleComp (spec₁ ++ₒ coeSuperSpec ++ₒ spec₃ ++ₒ spec₄) α := ↑oa
+-- example (oa : OracleComp ((spec₁ ++ₒ spec₂) ++ₒ (spec₃ ++ₒ coeSuperSpec)) α) :
+--   OracleComp (spec₁ ++ₒ spec₂ ++ₒ spec₃ ++ₒ coeSuperSpec) α := ↑oa
+
+-- /-- coercion makes it possible to mix computations on individual oracles -/
+-- example : OracleComp (unifSpec ++ₒ spec₁) Bool := do
+--   let n : Fin 315 ←$[0..314]; let m : Fin 315 ←$[0..314]
+--   if n = m then return true else coin
 
 end tests
